BoltLean/Domination.lean
@@ -1,0 +1,24 @@
+import BoltLean.Ltl
+
+namespace Formula
+def dominates (phi psi: Formula n): Prop :=
+  ∀ (t: Trace n), psi.eval t → phi.eval t
+
+
+theorem or_dominates (phi psi: Formula n) (f: Formula n):
+  phi.dominates psi → (f.Or phi).dominates (f.Or psi) := by
+    rw [dominates, dominates]
+    apply forall_imp
+    intro t h1 h2
+    simp [eval, eval_aux] at h2
+    simp [eval, eval_aux]
+    match h2 with
+    | ⟨hi, h_or⟩ => exists hi
+                    match h_or with
+                    | .inl hf => apply Or.inl; assumption
+                    | .inr h_psi => apply Or.inr
+                                    simp [eval, hi] at h1;
+                                    apply h1; assumption
+
+
+end Formula
